mppa_k1c/PostpassSchedulingProof.v
@@ -21,13 +21,23 @@ Require Import PostpassScheduling.
 (** * Relational characterization of the transformation *)
 
 Definition match_prog (p tp: Asmblock.program) :=
-  match_program (fun _ f tf => tf = transf_fundef f) eq p tp.
+  match_program (fun _ f tf => transf_fundef f = OK tf) eq p tp.
 
 Lemma transf_program_match:
-  forall p, match_prog p (transf_program p).
+  forall p tp, transf_program p = OK tp -> match_prog p tp.
 Proof.
-  intros. eapply match_transform_program; eauto.
+  intros. eapply match_transform_partial_program; eauto.
 Qed.
+
+Inductive transf_block_spec (ge: Genv.t fundef unit) (f: function) (bb tbb: bblock) :=
+  | transf_block_spec_intro:
+      (forall rs m,
+      exec_bblock ge f bb rs m = exec_bblock ge f tbb rs m) ->
+      transf_block_spec ge f bb tbb.
+
+Axiom transf_block_inv:
+  forall ge f bb tbb,
+  transf_block bb = OK tbb -> transf_block_spec ge f bb tbb.
 
 Section PRESERVATION.
 
@@ -39,59 +49,115 @@ Let tge := Genv.globalenv tprog.
 Lemma symbols_preserved:
   forall id,
   Genv.find_symbol tge id = Genv.find_symbol ge id.
-Proof (Genv.find_symbol_transf TRANSL).
+Proof (Genv.find_symbol_match TRANSL).
 
 Lemma senv_preserved:
   Senv.equiv ge tge.
-Proof (Genv.senv_transf TRANSL).
+Proof (Genv.senv_match TRANSL).
 
 Lemma functions_translated:
   forall v f,
   Genv.find_funct ge v = Some f ->
-  Genv.find_funct tge v = Some (transf_fundef f).
-Proof (Genv.find_funct_transf TRANSL).
+  exists tf,
+  Genv.find_funct tge v = Some tf /\ transf_fundef f = OK tf.
+Proof (Genv.find_funct_transf_partial TRANSL).
 
 Lemma function_ptr_translated:
   forall v f,
   Genv.find_funct_ptr ge v = Some f ->
-  Genv.find_funct_ptr tge v = Some (transf_fundef f).
-Proof (Genv.find_funct_ptr_transf TRANSL).
+  exists tf,
+  Genv.find_funct_ptr tge v = Some tf /\ transf_fundef f = OK tf.
+Proof (Genv.find_funct_ptr_transf_partial TRANSL).
+
+Lemma functions_transl:
+  forall fb f tf,
+  Genv.find_funct_ptr ge fb = Some (Internal f) ->
+  transf_function f = OK tf ->
+  Genv.find_funct_ptr tge fb = Some (Internal tf).
+Proof.
+  intros. exploit function_ptr_translated; eauto.
+  intros (tf' & A & B). monadInv B. rewrite H0 in EQ. inv EQ. auto.
+Qed.
 
 Inductive match_states: state -> state -> Prop :=
   | match_states_intro:
       forall s1 s2, s1 = s2 -> match_states s1 s2.
 
-(** TODO - continue *)
+Lemma prog_main_preserved:
+  prog_main tprog = prog_main prog.
+Proof (match_program_main TRANSL).
 
-(* Lemma transf_initial_states:
+Lemma prog_main_address_preserved:
+  (Genv.symbol_address (Genv.globalenv prog) (prog_main prog) Ptrofs.zero) =
+  (Genv.symbol_address (Genv.globalenv tprog) (prog_main tprog) Ptrofs.zero).
+Proof.
+  unfold Genv.symbol_address. rewrite symbols_preserved.
+  rewrite prog_main_preserved. auto.
+Qed.
+
+Lemma transf_initial_states:
   forall st1, initial_state prog st1 ->
   exists st2, initial_state tprog st2 /\ match_states st1 st2.
 Proof.
   intros. inv H.
   econstructor; split.
-  eapply initial_state_intro with (m0 := m0).
-  eapply (Genv.init_mem_transf TRANSL); eauto.
-(*   rewrite (match_program_main TRANSL), symbols_preserved; eauto.
-  apply function_ptr_translated; auto.
-  rewrite sig_function_translated. auto. *)
-  constructor; auto. constructor.
+  - eapply initial_state_intro.
+    eapply (Genv.init_mem_transf_partial TRANSL); eauto.
+  - econstructor; eauto. subst ge0. subst rs0. rewrite prog_main_address_preserved. auto.
 Qed.
 
 Lemma transf_final_states:
   forall st1 st2 r,
   match_states st1 st2 -> final_state st1 r -> final_state st2 r.
 Proof.
-  intros. inv H0. inv H. inv H5. econstructor; eauto.
+  intros. inv H0. inv H. econstructor; eauto.
 Qed.
 
-Theorem transf_program_correct:
-  forward_simulation (Linear.semantics prog) (Linear.semantics tprog).
+Lemma transf_find_bblock:
+  forall ofs f bb tf,
+  find_bblock (Ptrofs.unsigned ofs) (fn_blocks f) = Some bb ->
+  transf_function f = OK tf ->
+  exists tbb,
+    find_bblock (Ptrofs.unsigned ofs) (fn_blocks tf) = Some tbb
+    /\ transf_block bb = OK tbb.
 Proof.
-  eapply forward_simulation_opt.
-  apply senv_preserved.
-  eexact transf_initial_states.
-  eexact transf_final_states.
-  eexact transf_step_correct.
+Admitted.
+
+Lemma transf_exec_bblock:
+  forall f tf bb rs m rs' m',
+  exec_bblock ge f bb rs m = Next rs' m' ->
+  transf_function f = OK tf ->
+  exec_bblock tge tf bb rs m = Next rs' m'.
+Proof.
+Admitted.
+
+Axiom TODO: False.
+
+Theorem transf_step_correct:
+  forall s1 t s2, step ge s1 t s2 ->
+  forall s1' (MS: match_states s1 s1'),
+  (exists s2', step tge s1' t s2' /\ match_states s2 s2').
+Proof.
+  induction 1; intros; inv MS.
+  - exploit function_ptr_translated; eauto. intros (tf & A & B). monadInv B.
+    exploit transf_find_bblock; eauto. intros (tbb & C & D).
+    exists (State rs' m'); split; try (constructor; auto).
+    econstructor; eauto.
+    exploit transf_block_inv; eauto. intros E. inv E.
+    erewrite <- H3.
+    eapply transf_exec_bblock; eauto.
+  - destruct TODO.
+  - destruct TODO.
+Admitted.
+
+Theorem transf_program_correct:
+  forward_simulation (Asmblock.semantics prog) (Asmblock.semantics tprog).
+Proof.
+  eapply forward_simulation_step.
+  - apply senv_preserved.
+  - apply transf_initial_states.
+  - apply transf_final_states.
+  - apply transf_step_correct.
 Qed.
- *)
+
 End PRESERVATION.
